```agda
module cgp.Word where

import cgp.RE as RE
open RE using (RE; Ï• ; Îµ ; $_`_ ; _â—_`_ ; _+_`_ ; _*_`_ ; Îµâˆ‰ ; Îµâˆˆ ; Îµâˆˆ_+_  ; Îµâˆˆ_<+_ ; Îµâˆˆ_+>_ ; Îµâˆˆ_â—_ ; Îµâˆˆ*  ; ÎµâˆˆÎµ ; Îµâˆ‰râ†’Â¬Îµâˆˆr ; Îµâˆ‰fst ; Îµâˆ‰snd ; Îµâˆ‰$ ; Îµâˆ‰_+_)

import Data.List as List
open List using (List ; _âˆ·_ ; [] ; _++_ ; [_]; map; concatMap )

import Data.Char as Char
open Char using (Char)

import Data.Nat as Nat
open Nat using ( â„• ; suc ; zero )


import Relation.Binary.PropositionalEquality as Eq
open Eq using (_â‰¡_; refl; trans; sym; cong; cong-app; subst)
-- open Eq.â‰¡-Reasoning using (begin_; step-â‰¡;  step-â‰¡-âˆ£;  step-â‰¡-âŸ©; _âˆ)

import Relation.Nullary as Nullary 
import Relation.Nullary.Negation using (contradiction; contraposition)

open Nullary using (Â¬_)

open import Function using (_âˆ˜_)

```


### Defintion 5 : Word
A word is a sequence of literals.

 w :: = [] | â„“ âˆ· w

We represent a word as a list of characters in Agda. 


### Definition 6 : word-regexp membership relation w âˆˆ âŸ¦ r âŸ§ 

Let w be word, r be regular expression, we define the membership relationship as follows

  [] âˆˆ âŸ¦ Îµ âŸ§ 

  â„“  âˆˆ âŸ¦ â„“ âŸ§


  xs âˆˆ âŸ¦ l âŸ§
  ys âˆˆ âŸ¦ r âŸ§
 ----------------------
  xs ++ ys âˆˆ âŸ¦ l â— r âŸ§ 

  xs âˆˆ âŸ¦ l âŸ§
  --------------
  xs âˆˆ âŸ¦ l + r âŸ§


  ys âˆˆ âŸ¦ r âŸ§
  --------------
  ys âˆˆ âŸ¦ l + r âŸ§

  xs âˆˆ âŸ¦ Îµ + (r â— r*) âŸ§ 
  ---------------------
  xs âˆˆ âŸ¦ r * âŸ§ 


```agda
data _âˆˆâŸ¦_âŸ§ : List Char â†’ RE â†’ Set where
  Îµ      : [] âˆˆâŸ¦ Îµ âŸ§
  $_      : âˆ€ { loc : â„• } ( c : Char ) â†’ [ c ] âˆˆâŸ¦ $ c ` loc âŸ§ 
  _â—_â§º_  : âˆ€ {xs ys zs : List Char} { l r : RE } { loc : â„• }
        â†’ xs âˆˆâŸ¦ l âŸ§
        â†’ ys âˆˆâŸ¦ r âŸ§
        â†’ xs ++ ys â‰¡ zs            -- this evidence is essential, without which the pair case in the unflat will not type-check, why?
        ------------------------- 
        â†’ zs âˆˆâŸ¦ l â— r ` loc âŸ§
  _+L_   : âˆ€ { l : RE } {xs : List Char} { loc : â„• } ( r : RE )
        â†’ xs âˆˆâŸ¦ l âŸ§
        -------------------------
        â†’ xs âˆˆâŸ¦ l + r ` loc  âŸ§
  _+R_ : âˆ€ { r : RE } {xs : List Char} { loc : â„• } ( l : RE )
        â†’ xs âˆˆâŸ¦ r âŸ§
        -------------------------
        â†’ xs âˆˆâŸ¦ l + r ` loc âŸ§        
  _*   : âˆ€ { r : RE } { nÎµ : Îµâˆ‰ r } { xs : List Char } { loc : â„• } 
        â†’ xs âˆˆâŸ¦ Îµ + (r â— (r * nÎµ ` loc ) ` loc ) ` loc  âŸ§
        --------------------------
        â†’ xs âˆˆâŸ¦ r * nÎµ ` loc  âŸ§

```  


> KL: The above definition is adopted from [1], except that the quantifers (for the constructors) were missing from [1].


An interesting observation is that the above definition is phrased in a deduction system, which is unlike the convention, in which we first
 define the mapping from regular expressions to sets of words, then the test can be expressed in terms of a set member test.


Definition 6':  ğ“›( r ) mapping regular expression to set of strings

â„’( r ), the language of r, defines the set of all string inhabiting in r.

   â„’( Ï• ) = {}
   â„’( Îµ ) = { [] }
   â„’( â„“ ) = { â„“ âˆ· [] }
   â„’( l â— r ) = { wâ‚ ++ wâ‚‚ | wâ‚ âˆˆ â„’( l ) âˆ§ wâ‚‚ âˆˆ â„’( r ) }
   â„’( l + r ) = â„’( l ) âˆª â„’( r )
   â„’( r * )   = { wâ‚ ++ ... ++ wâ‚™ | n â‰¥ 0 âˆ§ wáµ¢ âˆˆ â„’( r ) âˆ§ i âˆˆ {1,...,n} }

   then
   w âˆˆâŸ¦ r âŸ§ can be defined as w âˆˆ â„’( r ) where _âˆˆ_ is the set member relation.
   
### TODO: can we implement the above in agda?
If so, can we show that w âˆˆâŸ¦ r âŸ§ iff w âˆˆ â„’( r )

> KL: Conjecture, to do so we need a lazy set, ğ“›( r ) maps r to a lazy set.
> The _âˆˆ_ test must be done coinductively, otherwise b âˆˆ ğ“›( a* ) won't terminate.


#### Sub Lemma 6.1 ( empty word inhabitance implies negation of non-nullability )

Let r be a non problematic regular expression.
Let [] âˆˆ âŸ¦ r âŸ§.
Then Â¬ ( Îµâˆ‰ r ).

```agda
[]âˆˆâŸ¦râŸ§â†’Â¬Îµâˆ‰r : âˆ€ { r : RE } â†’ [] âˆˆâŸ¦ r âŸ§  â†’ Â¬ ( Îµâˆ‰ r )
[]âˆˆâŸ¦râŸ§â†’Â¬Îµâˆ‰r {Îµ} = Î» x Îµâˆ‰Îµ â†’  (Îµâˆ‰râ†’Â¬Îµâˆˆr Îµâˆ‰Îµ) ÎµâˆˆÎµ
[]âˆˆâŸ¦râŸ§â†’Â¬Îµâˆ‰r {$ c ` loc } = Î»()
[]âˆˆâŸ¦râŸ§â†’Â¬Îµâˆ‰r { s â— t ` loc } (  _â—_â§º_ {[]} {[]} {[]} {s} {t} {loc} []âˆˆs []âˆˆt eq ) Îµâˆ‰sâ—t with  Îµâˆ‰sâ—t
...                         | Îµâˆ‰fst  Îµâˆ‰s = ([]âˆˆâŸ¦râŸ§â†’Â¬Îµâˆ‰r  []âˆˆs) Îµâˆ‰s
...                         | Îµâˆ‰snd  Îµâˆ‰t = ([]âˆˆâŸ¦râŸ§â†’Â¬Îµâˆ‰r  []âˆˆt) Îµâˆ‰t
[]âˆˆâŸ¦râŸ§â†’Â¬Îµâˆ‰r { s + t ` loc } (  _+L_ {s} {[]} {loc} t []âˆˆs ) Îµâˆ‰s+t with Îµâˆ‰s+t
...                         | Îµâˆ‰ Îµâˆ‰s + Îµâˆ‰t = ([]âˆˆâŸ¦râŸ§â†’Â¬Îµâˆ‰r  []âˆˆs) Îµâˆ‰s
[]âˆˆâŸ¦râŸ§â†’Â¬Îµâˆ‰r { s + t ` loc } (  _+R_ {t} {[]} {loc} s []âˆˆt ) Îµâˆ‰s+t with Îµâˆ‰s+t
...                         | Îµâˆ‰ Îµâˆ‰s + Îµâˆ‰t = ([]âˆˆâŸ¦râŸ§â†’Â¬Îµâˆ‰r  []âˆˆt) Îµâˆ‰t
[]âˆˆâŸ¦râŸ§â†’Â¬Îµâˆ‰r { s * Îµâˆ‰s ` loc } ( _* {s} {Îµâˆ‰s} {[]} {loc} []âˆˆÎµ+sâ—s* )  Îµâˆ‰s* =  (Îµâˆ‰râ†’Â¬Îµâˆˆr Îµâˆ‰s*) Îµâˆˆ* 


[]âˆˆâŸ¦râŸ§â†’Îµâˆˆr : âˆ€ { r : RE } â†’ [] âˆˆâŸ¦ r âŸ§ â†’ Îµâˆˆ r
[]âˆˆâŸ¦râŸ§â†’Îµâˆˆr = RE.Â¬Îµâˆ‰râ†’Îµâˆˆr âˆ˜ []âˆˆâŸ¦râŸ§â†’Â¬Îµâˆ‰r 
```

```agda
-- aux lemma needed for proving sub lemma in partial-derivatives, such as Â¬recons-[]-from-pdinstance-star
Â¬câˆ·wâ‰¡[] : âˆ€ { c : Char } { w : List Char } â†’ Â¬ c âˆ· w â‰¡ []
Â¬câˆ·wâ‰¡[] {c} {w} = Î»()

```

```agda
{-
import Data.Product as Product
open Product using (Î£; _,_; âˆƒ; Î£-syntax; âˆƒ-syntax; _Ã—_ )
open Î£ using (projâ‚ ; projâ‚‚)

import Relation.Nullary.Decidable as Decidable
open Decidable using
  ( Dec; yes; no; âŒŠ_âŒ‹; True; toWitness; fromWitness; _Ã—-dec_; _âŠ-dec_; Â¬?)

postulate
  enum : ( r : RE ) â†’ ( w : List Char ) â†’ List ( w âˆˆâŸ¦ r âŸ§ )
-}  
{-  
enum Ï• _ = []
enum Îµ [] = [  Îµ ]
enum Îµ (_ âˆ· _) = [] 
enum ($ c ` loc ) [] = []
enum ($ c ` loc ) (c' âˆ· []) with c Char.â‰Ÿ c'
...                            | yes refl = [ $ c' ]
...                            | no  _    = []
enum ($ c ` loc ) (c' âˆ· cs) = []
-}
{-
enum (l â— r ` loc ) xs  =
  let n = List.length xs
      ps = List.upTo n
      xxs = map (Î» p â†’ List.splitAt p xs ) ps
  in concatMap (Î» { yzs â†’
                      let ysâˆˆls = enum l (projâ‚ yzs)
                          zsâˆˆrs = enum r (projâ‚‚ yzs)
                      in concatMap (Î» ysâˆˆl â†’ (List.map (Î» zsâˆˆr â†’ ( ysâˆˆl â— zsâˆˆr â§º refl ) ) zsâˆˆrs ) ) ysâˆˆls } ) xxs
-}    


```
